rel.v
@@ -26,20 +26,43 @@ Next Obligation. cbv. firstorder. Qed.
 Instance Involution_converse {A}: Involution (@converse A).
 Proof. now intros ? ?. Qed.
 
-(** provided that [const eq], [square], and [converse] are below [t], 
-    we have that [gfp b], [t R], [bt R] and [T f R] are always equivalence relations. *)
-(* TOTHINK: also [b (T f R)], useful? *)
 Section s.
   Variables (A: Type) (b: mon (relation A)).
-  Hypothesis eq_t: const eq <= t b.
-  Hypothesis square_t: square <= t b.
-  Lemma PreOrder_T f R: PreOrder (t (B b) f R).
+  Notation t := (t b).
+  Notation T := (T b).
+  Notation bt := (bt b).
+  Notation bT := (bT b).
+
+  (** [gfp] is always a subrelation of [t R], [bt R], [T f R], and [bT f R] 
+      TOTHINK: declare other links in the lattice?
+      (bt<=bT<=T and bt<=t<=T)
+   *)
+  Global Instance subrelation_gfp_T f (R: relation A): subrelation (gfp b) (T f R).
+  Proof. refine (gfp_T _ _ R). Qed.
+  
+  Global Instance subrelation_gfp_t (R: relation A): subrelation (gfp b) (t R).
+  Proof. refine (gfp_t _ R). Qed.
+
+  (** the next two are not declared as instances by default, 
+      in order to circumvent setoid_rewriting inefficiencies *)
+  Lemma subrelation_gfp_bt (R: relation A): subrelation (gfp b) (bt R).
+  Proof. refine (gfp_bt _ R). Qed.
+  
+  Lemma subrelation_gfp_bT f (R: relation A): subrelation (gfp b) (bT f R).
+  Proof. refine (gfp_bT _ _ R). Qed.
+
+  (** provided that [const eq], [square], and [converse] are below [t], 
+    we have that [gfp b], [t R], [bt R], [T f R], and [bT f R] are always equivalence relations. *)
+  (* TOTHINK: setup typclasses to avoid repetitions? *)
+  Hypothesis eq_t: const eq <= t.
+  Hypothesis square_t: square <= t.
+  Lemma PreOrder_T f R: PreOrder (T f R).
   Proof.
     constructor.
-    intro. now apply (ftT_T f eq_t).
-    intros ? y ???. apply (ftT_T f square_t). exists y; assumption.
+    intro. now apply (fT_T eq_t).
+    intros ? y ???. apply (fT_T square_t). exists y; assumption.
   Qed.
-  Lemma PreOrder_t R: PreOrder (t b R).
+  Lemma PreOrder_t R: PreOrder (t R).
   Proof.
     constructor.
     intro. now apply (ft_t eq_t).
@@ -47,22 +70,28 @@ Section s.
   Qed.
   Corollary PreOrder_gfp: PreOrder (gfp b).
   Proof PreOrder_t bot.
-  Lemma PreOrder_bt R: PreOrder (bt b R).
+  Lemma PreOrder_bt R: PreOrder (bt R).
   Proof.
     constructor.
     intro. now apply (fbt_bt eq_t).
     intros ? y ???. apply (fbt_bt square_t). exists y; assumption.
   Qed.
-
-  Hypothesis converse_t: converse <= t b.
-  Lemma Equivalence_T f R: Equivalence (t (B b) f R).
+  Lemma PreOrder_bT f R: PreOrder (bT f R).
   Proof.
     constructor.
-    intro. now apply (ftT_T f eq_t).
-    intros x y. apply (ftT_T f converse_t).
-    intros ? y ???. apply (ftT_T f square_t). exists y; assumption.
+    intro. now apply (fbT_bT eq_t).
+    intros ? y ???. apply (fbT_bT square_t). exists y; assumption.
   Qed.
-  Lemma Equivalence_t R: Equivalence (t b R).
+
+  Hypothesis converse_t: converse <= t.
+  Lemma Equivalence_T f R: Equivalence (T f R).
+  Proof.
+    constructor.
+    intro. now apply (fT_T eq_t).
+    intros x y. apply (fT_T converse_t f).
+    intros ? y ???. apply (fT_T square_t). exists y; assumption.
+  Qed.
+  Lemma Equivalence_t R: Equivalence (t R).
   Proof.
     constructor.
     intro. now apply (ft_t eq_t).
@@ -71,28 +100,21 @@ Section s.
   Qed.
   Corollary Equivalence_gfp: Equivalence (gfp b).
   Proof Equivalence_t bot.
-  Lemma Equivalence_bt R: Equivalence (bt b R).
+  Lemma Equivalence_bt R: Equivalence (bt R).
   Proof.
     constructor.
     intro. now apply (fbt_bt eq_t).
     intros x y. apply (fbt_bt converse_t).
     intros ? y ???. apply (fbt_bt square_t). exists y; assumption.
   Qed.
+  Lemma Equivalence_bT f R: Equivalence (bT f R).
+  Proof.
+    constructor.
+    intro. now apply (fbT_bT eq_t).
+    intros x y. apply (fbT_bT converse_t).
+    intros ? y ???. apply (fbT_bT square_t). exists y; assumption.
+  Qed.
 End s.
-
-
-(** [gfp] is always a subrelation of [t R], [bt R] and [T f R] *)
-Instance rel_gfp_T A b f (R: relation A): subrelation (gfp b) (t (B b) f R).
-Proof. refine (gfp_T _ f R). Qed.
-
-Instance rel_gfp_t A b (R: relation A): subrelation (gfp b) (t b R).
-Proof. refine (gfp_t _ R). Qed.
-
-Instance rel_gfp_bt A b (R: relation A): subrelation (gfp b) (bt b R).
-Proof.
-  intros x y H. apply (gfp_pfp b) in H.
-  revert H. apply b. apply rel_gfp_t.
-Qed.
 
 
 (** * Contexts *)
@@ -123,13 +145,23 @@ Global Opaque unary_ctx.
 Lemma unary_sym S (f: S -> S): compat converse (unary_ctx f).
 Proof. intro R. simpl. apply leq_unary_ctx. intros. now apply in_unary_ctx. Qed.
 
-(** if it is below [t], then the function [f] always preserves [t R] and [bt R]*)
-Lemma unary_proper S (f: S -> S) b:
+(** if it is below [t], then the function [f] always preserves [t R], [bt R], [T f R], [bT f R] *)
+Lemma unary_proper_t S (f: S -> S) b:
   unary_ctx f <= t b -> forall R, Proper (t b R ==> t b R) f.
 Proof. intros H R x x' Hx. apply (ft_t H). now apply (in_unary_ctx f). Qed.
 Lemma unary_proper_bt S (f: S -> S) b:
   unary_ctx f <= t b -> forall R, Proper (bt b R ==> bt b R) f.
 Proof. intros H R x x' Hx. apply (fbt_bt H). now apply (in_unary_ctx f). Qed.
+Lemma unary_proper_T S (f: S -> S) b g:
+  unary_ctx f <= t b -> forall R, Proper (T b g R ==> T b g R) f.
+Proof. intros H R x x' Hx. apply (fT_T H). now apply (in_unary_ctx f). Qed.
+Lemma unary_proper_bT S (f: S -> S) b g:
+  unary_ctx f <= t b -> forall R, Proper (bT b g R ==> bT b g R) f.
+Proof. intros H R x x' Hx. apply (fbT_bT H). now apply (in_unary_ctx f). Qed.
+
+Global Instance unary_proper_Tctx S (f: S -> S) b R:
+  Proper (T b (unary_ctx f) R ==> T b (unary_ctx f) R) f.
+Proof. intros x x' Hx. apply (fTf_Tf b). now apply (in_unary_ctx f). Qed.
 
                                  
 (** binary context: [unary_ctx f](R) = {(f x x', f y y') | x R y, x' R y' }  *)
@@ -160,13 +192,23 @@ Global Opaque binary_ctx.
 Lemma binary_sym S (f: S -> S -> S): compat converse (binary_ctx f).
 Proof. intro R. simpl. apply leq_binary_ctx. intros. now apply in_binary_ctx. Qed.
 
-(** if it is below [t], then the function [f] always preserves [t R] *)
-Lemma binary_proper S (f: S -> S -> S) b:
+(** if it is below [t], then the function [f] always preserves [t R], [bt R], [T f R], [bT f R] *)
+Lemma binary_proper_t S (f: S -> S -> S) b:
   binary_ctx f <= t b -> forall R, Proper (t b R ==> t b R ==> t b R) f.
 Proof. intros H R x x' Hx y y' Hy. apply (ft_t H). now apply (in_binary_ctx f). Qed.
 Lemma binary_proper_bt S (f: S -> S -> S) b:
   binary_ctx f <= t b -> forall R, Proper (bt b R ==> bt b R ==> bt b R) f.
 Proof. intros H R x x' Hx y y' Hy. apply (fbt_bt H). now apply (in_binary_ctx f). Qed.
+Lemma binary_proper_T S (f: S -> S -> S) b g:
+  binary_ctx f <= t b -> forall R, Proper (T b g R ==> T b g R ==> T b g R) f.
+Proof. intros H R x x' Hx y y' Hy. apply (fT_T H). now apply (in_binary_ctx f). Qed.
+Lemma binary_proper_bT S (f: S -> S -> S) b g:
+  binary_ctx f <= t b -> forall R, Proper (bT b g R ==> bT b g R ==> bT b g R) f.
+Proof. intros H R x x' Hx y y' Hy. apply (fbT_bT H). now apply (in_binary_ctx f). Qed.
+
+Global Instance binary_proper_Tctx S (f: S -> S -> S) b R:
+  Proper (T b (binary_ctx f) R ==> T b (binary_ctx f) R ==> T b (binary_ctx f) R) f.
+Proof. intros x x' Hx y y' Hy. apply (fTf_Tf b). now apply (in_binary_ctx f). Qed.
 
                                  
 (** ternary context: [unary_ctx f](R) = {(f x x', f y y') | x R y, x' R y' }  *)
@@ -200,14 +242,23 @@ Global Opaque ternary_ctx.
 Lemma ternary_sym S (f: S -> S -> S -> S): compat converse (ternary_ctx f).
 Proof. intro R. simpl. apply leq_ternary_ctx. intros. now apply in_ternary_ctx. Qed.
 
-(** if it is below [t], then the function [f] always preserves [t R] and [bt R] *)
-Lemma ternary_proper S (f: S -> S -> S -> S) b:
+(** if it is below [t], then the function [f] always preserves [t R], [bt R], [T f R], [bT f R] *)
+Lemma ternary_proper_t S (f: S -> S -> S -> S) b:
   ternary_ctx f <= t b -> forall R, Proper (t b R ==> t b R ==> t b R ==> t b R) f.
 Proof. intros H R x x' Hx y y' Hy z z' Hz. apply (ft_t H). now apply (in_ternary_ctx f). Qed.
 Lemma ternary_proper_bt S (f: S -> S -> S -> S) b:
   ternary_ctx f <= t b -> forall R, Proper (bt b R ==> bt b R ==> bt b R ==> bt b R) f.
 Proof. intros H R x x' Hx y y' Hy z z' Hz. apply (fbt_bt H). now apply (in_ternary_ctx f). Qed.
+Lemma ternary_proper_T S (f: S -> S -> S -> S) b g:
+  ternary_ctx f <= t b -> forall R, Proper (T b g R ==> T b g R ==> T b g R ==> T b g R) f.
+Proof. intros H R x x' Hx y y' Hy z z' Hz. apply (fT_T H). now apply (in_ternary_ctx f). Qed.
+Lemma ternary_proper_bT S (f: S -> S -> S -> S) b g:
+  ternary_ctx f <= t b -> forall R, Proper (bT b g R ==> bT b g R ==> bT b g R ==> bT b g R) f.
+Proof. intros H R x x' Hx y y' Hy z z' Hz. apply (fbT_bT H). now apply (in_ternary_ctx f). Qed.
 
+Global Instance ternary_proper_Tctx S (f: S -> S -> S -> S) b R:
+  Proper (T b (ternary_ctx f) R ==> T b (ternary_ctx f) R ==> T b (ternary_ctx f) R ==> T b (ternary_ctx f) R) f.
+Proof. intros x x' Hx y y' Hy z z' Hz. apply (fTf_Tf b). now apply (in_ternary_ctx f). Qed.
 
 Transparent pair.
 Lemma converse_pair A (p q: A): converse (pair p q) == pair q p.
